poSTVM/poSTVM_state_alt.thy
@@ -734,4 +734,6 @@ definition get_func_by_name :: "model_state \<Rightarrow> func_name \<Rightarrow
 declare get_func_by_name_def [simp] 
 
 declare fmupd_reorder_neq [simp]
+(*declare fmran_def [simp]
+declare ffold_def [simp]*)
 end
